Add another proof method to obtain partial correctness, and use it to prove Abs

Correctness/Correctness.lean
@@ -21,6 +21,8 @@ open Spec' (cut assert)
 open Iterate (iterate iterate_eq)
 open Classical
 
+----------------------------------------------------------------------
+
 theorem not_forall_eq_exists_not (p : α → Prop) : (¬ ∀ x, p x) = ∃ x, ¬ p x := by
   apply propext
   constructor
@@ -35,29 +37,51 @@ theorem not_forall_eq_exists_not (p : α → Prop) : (¬ ∀ x, p x) = ∃ x, ¬
     have := h₂ a
     contradiction
 
-/- Result from page 2: I1, I2, I3 implies Partial Correctness. -/
-theorem by_inv [Sys σ] [Spec σ] (inv : σ → Prop)
-    (ini  : ∀ s0, pre s0 → inv s0)  -- I1
-    (step : ∀ s, inv s → ¬ exit s → inv (next s)) -- I2
-    (stop : ∀ s0 sf, inv sf → exit sf → post s0 sf)  -- I3
+----------------------------------------------------------------------
+
+/--
+Prove partial correctness using stepwise invariants.
+
+We use `s0`, `si`, and `sf` to refer to initial, intermediate, and
+final (exit) states respectively.
+
+This is the result from page 2 of the paper. Note that the `inv`
+function must specify an invariant for _each_ machine instruction,
+which makes this proof method tedious to use for larger programs.
+
+Also see `partial_correctness_from_verification_conditions` and
+`partial_correctness_from_assertions`.
+-/
+theorem partial_correctness_by_stepwise_invariants [Sys σ] [Spec σ] (inv : σ → σ → Prop)
+    (ini  : ∀ s0, pre s0 → inv s0 s0)  -- I1
+    (step : ∀ s0 si, inv s0 si → ¬ exit si → inv s0 (next si)) -- I2
+    (stop : ∀ s0 sf, inv s0 sf → exit sf → post s0 sf)  -- I3
     : PartialCorrectness σ :=
-  fun s n hp he =>
-    let rec find (i : Nat) (h : inv (run s i)) (hle : i ≤ n)
-            : ∃ m : Nat, m ≤ n ∧ exit (run s m) ∧ post s (run s m) :=
+  fun s0 n hp he =>
+    let rec find (i : Nat) (h : inv s0 (run s0 i)) (hle : i ≤ n)
+            : ∃ m : Nat, m ≤ n ∧ exit (run s0 m) ∧ post s0 (run s0 m) :=
       if hn : i < n then
-        if he : exit (run s i) then
+        if he : exit (run s0 i) then
           ⟨i, Nat.le_of_lt hn, he, stop _ _ h he⟩
         else
-          have : inv (run s (i+1)) := by
-            rw [← next_run]; exact step _ h he
+          have : inv s0 (run s0 (i+1)) := by
+            rw [← next_run]; exact step _ _ h he
           find (i+1) this hn
       else
         have := Nat.ge_of_not_lt hn
         have := Nat.le_antisymm this hle
-        have hinv : inv (run s n) := by subst this; assumption
-        have hpost : post s (run s n) := stop _ _ hinv he
+        have hinv : inv s0 (run s0 n) := by subst this; assumption
+        have hpost : post s0 (run s0 n) := stop _ _ hinv he
         ⟨n, Nat.le_refl _, he, hpost⟩
     find 0 (ini _ hp) (Nat.zero_le _)
+
+----------------------------------------------------------------------
+
+-- Prove partial correctness using inductive assertions using the
+-- functions `csteps` (to characterize the number of steps to reach
+-- the next cutpoint) and `nextc` (to characterize the next cutpoint
+-- state). Note that the function `csteps` is partial: if no cutpoint
+-- is reachable from `s`, then the recursion does not terminate.
 
 noncomputable def csteps [Sys σ] [Spec' σ] (s : σ) (i : Nat) : Nat :=
   iterate (fun (s, i) => if cut s then .inl i else .inr (next s, i + 1)) (s, i)
@@ -110,10 +134,10 @@ theorem csteps_not_cut [Sys σ] [Spec' σ] {s : σ} (h₁ : ¬ cut s)
   assumption
 
 /--
-Helper theorem. Given a state `s` and `cut (run s n)` for `n`, then there is
-`k` such that `csteps s 0 = k` and `k ≤ n`.
-Note that `cut (run s n)` ensures `csteps s 0` terminates because we will find a
-`cut` in at most `n` steps.
+Helper theorem. Given a state `s` and `cut (run s n)` for `n`, then
+there is `k` such that `csteps s 0 = k` and `k ≤ n`.
+Note that `cut (run s n)` ensures `csteps s 0` terminates because we
+will find a `cut` in at most `n` steps.
 -/
 theorem find_next_cut [Sys σ] [Spec' σ] (s : σ) (hc : cut (run s n)) :
   ∃ k : Nat, csteps s 0 = k ∧ k ≤ n ∧ cut (run s k) :=
@@ -133,10 +157,23 @@ theorem find_next_cut [Sys σ] [Spec' σ] (s : σ) (hc : cut (run s n)) :
   loop s 0 (Nat.zero_le ..) rfl
 
 /--
-Theorem 1 from page 5. If V1-V4 hold, then we have partial correctness.
+Prove partial correctness using inductive assertions and functions
+`csteps` and `nextc`.
 
-We use `s0`, `si`, and `sf` to refer to initial, intermediate, and final (exit)
-states respectively.
+We use `s0`, `si`, and `sf` to refer to initial, intermediate, and
+final (exit) states respectively.
+
+This is Theorem 1 from page 5 of the paper. This proof method is more
+convenient to use than `partial_correctness_by_stepwise_invariants`
+because we need only attach assertions at certain cutpoints. However,
+it may still be tedious to use from the point of view of automation
+because it is difficult to both symbolically simulate an instruction
+and unwind `csteps` in tandem. So far, we have found that it is
+easiest to determine what concrete value `csteps` yields (via symbolic
+simulation), and then perform symbolic simulation -- however, then we
+end up doing simulation twice, which is expensive.
+
+Also see `partial_correctness_from_assertions`.
 -/
 theorem partial_correctness_from_verification_conditions [Sys σ] [Spec' σ]
     (v1 : ∀ s0 : σ, pre s0 → assert s0 s0)
@@ -164,6 +201,177 @@ theorem partial_correctness_from_verification_conditions [Sys σ] [Spec' σ]
             rw [nextc, next_run, hk, run_run] at this
             simp [hck] at this
             assumption
+          have : n - (i + 1 + k) < n - i := by
+            apply Nat.sub_lt_sub_left; assumption; simp_arith
+          find (i + 1 + k) h' hle'
+      else
+        have := Nat.ge_of_not_lt hn
+        have := Nat.le_antisymm this hle
+        have ha : assert s0 (run s0 n) := by subst this; assumption
+        have hpost : post s0 (run s0 n) := v3 _ _ ha hexit
+        ⟨n, Nat.le_refl _, hexit, hpost⟩
+    find 0 (v1 s0 hp) (Nat.zero_le ..)
+
+----------------------------------------------------------------------
+
+-- Prove partial correctness using inductive assertions using the
+-- function `cassert` that checks if `assert` holds if at a cutpoint
+-- state, or else recurs until it hits one. This function is also
+-- partial: if no cutpoint is reachable, the recursion doesn't
+-- terminate.
+
+/--
+`cassert s0 si i`: if this function terminates, it returns a pair,
+whose first element is a `Nat = (i + the number of steps simulated
+from `si` to reach the next cutpoint)`, and the second element is a
+`Prop` that checks whether `assert` holds at that cutpoint state.
+-/
+noncomputable def cassert [Sys σ] [Spec' σ] (s0 si : σ) (i : Nat) : Nat × Prop :=
+  iterate (fun (si, i) => if cut si then .inl (i, assert s0 si) else .inr (next si, i + 1)) (si, i)
+
+theorem cassert_eq [Sys σ] [Spec' σ] (s0 si : σ) (i : Nat)
+        : cassert s0 si i = if cut si then (i, assert s0 si)
+                       else cassert s0 (next si) (i + 1) := by
+  unfold cassert
+  conv => lhs; rw [iterate_eq]
+  by_cases cut si <;> simp [*]
+  done
+
+theorem cassert_cut [Sys σ] [Spec' σ] {s0 si : σ} (h : cut si) (i : Nat) :
+  (cassert s0 si i).fst = i ∧
+  (cassert s0 si i).snd = assert s0 si := by
+  rw [cassert_eq]
+  simp [*]
+  done
+
+theorem cassert_not_cut [Sys σ] [Spec' σ] {s0 si : σ} (h₁ : ¬ cut si)
+  (h₂ : (cassert s0 (next si) (i+1)).fst = j) :
+  (cassert s0 si i).fst = j ∧
+  (cassert s0 si i).snd = (cassert s0 (next si) (i + 1)).snd := by
+  rw [cassert_eq]
+  simp [h₁]
+  assumption
+  done
+
+theorem cassert_lower_bound [Sys σ] [Spec' σ] {s0 si : σ} (n : Nat)
+  (h0 : cut (run si n))
+  (h1 : (cassert s0 si i).fst = j) :
+  i <= j := by
+  induction n generalizing i si
+  case zero =>
+    unfold run at h0
+    rw [cassert_eq] at h1
+    simp_all only [ite_true, Nat.le_refl]
+  case succ =>
+    rename_i _ _ n' h_inv
+    rw [run_succ] at h0
+    rw [cassert_eq] at h1
+    split at h1
+    · omega
+    · have h_inv' := @h_inv (i + 1) (next si) h0 h1
+      omega
+  done
+
+theorem find_next_cut_for_cassert [Sys σ] [Spec' σ] (s0 si : σ) (hc : cut (run si n)) :
+  ∃ k : Nat, (cassert s0 si 0).fst = k ∧
+             (cassert s0 si 0).snd = assert s0 (run si k) ∧
+             k ≤ n ∧
+             cut (run si k) :=
+  let rec loop (s' : σ) (i : Nat) (hle : i ≤ n) (heq : s' = run si i) :
+    ∃ k : Nat, (cassert s0 s' i).fst = k ∧
+               (cassert s0 s' i).snd = assert s0 (run s' (k - i)) ∧
+                k ≤ n ∧ cut (run si k) :=
+     if hn : i < n then
+       if hc : cut s' then
+         have := cassert_cut hc i
+         have h_i_i : i - i = 0 := by simp only [Nat.sub_self]
+         ⟨i, this.left, h_i_i ▸ this.right, hle, by subst s'; assumption⟩
+       else
+         have ⟨k, hs, hkn, hck⟩ := loop (next s') (i+1) hn (by simp [heq, run_succ'])
+         have h_not_cut := (cassert_not_cut hc hs).right
+         have : (cassert s0 s' i).snd = assert s0 (run s' (k - i)) := by
+          simp only [h_not_cut, hkn]
+          have h_next_cut : cut (run (next s') (n - i - 1)) := by
+            rw [heq]
+            have : (next (run si i)) = run (run si i) 1 := by
+              simp only [run]
+            simp only [this]
+            have : (run (run (run si i) 1) (n - i - 1)) = run si n := by
+              repeat (rw [run_run])
+              have : (i + (1 + (n - i - 1))) = n := by omega
+              rw [this]
+              done
+            simpa only [this]
+          have h_lb := @cassert_lower_bound _ (i + 1) k _ _ s0
+                        (next s') (n - i - 1) h_next_cut hs
+          conv =>
+            rhs
+            unfold run
+          have h_k_i : ¬ k - i = 0 := by omega
+          split
+          · contradiction
+          · rename_i x y h_k_i_y
+            simp at h_k_i_y
+            have : (k - (i + 1)) = k - i - 1 := by omega
+            simp [this, h_k_i_y]
+          done
+         ⟨k, (cassert_not_cut hc hs).left, this, hck.left, hck.right⟩
+     else
+       have hin : i = n := by omega
+       have h_left : (cassert s0 s' i).fst = n := by
+          have := @cassert_cut _ _ _ s0 _ hc n
+          subst hin
+          rw [heq]
+          simp only [this]
+       have h_right : (cassert s0 s' i).snd = assert s0 (run s' (n - i)) := by
+        simp only [Nat.sub_self, eq_iff_iff]
+        have := @cassert_cut _ _ _ s0 _ hc
+        subst hin
+        rw [heq]
+        simp only [this, Nat.sub_self, eq_iff_iff, run]
+        done
+       ⟨n, h_left, h_right, Nat.le_refl .., by assumption⟩
+  loop si 0 (Nat.zero_le ..) rfl
+
+
+/--
+Prove partial correctness from inductive assertions using `cassert`
+function.
+
+We use `s0`, `si`, and `sf` to refer to initial, intermediate, and
+final (exit) states respectively.
+
+This is more convenient to use that
+`partial_correctness_from_inductive_assertions` because we can do
+symbolic simulation and open `cassert` in tandem.
+-/
+theorem partial_correctness_from_assertions [Sys σ] [Spec' σ]
+    (v1 : ∀ s0 : σ, pre s0 → assert s0 s0)
+    (v2 : ∀ sf : σ, exit sf → cut sf)
+    (v3 : ∀ s0 sf : σ, assert s0 sf → exit sf → post s0 sf)
+    (v4 : ∀ s0 si : σ, assert s0 si → ¬ exit si → (cassert s0 (run si 1) 0).snd)
+    : PartialCorrectness σ :=
+    fun s0 n hp hexit =>
+    let rec find (i : Nat) (h : assert s0 (run s0 i)) (hle : i ≤ n) :
+                 ∃ m : Nat, m ≤ n ∧ exit (run s0 m) ∧ post s0 (run s0 m) :=
+      if hn : i < n then
+        if he : exit (run s0 i) then
+          ⟨i, Nat.le_of_lt hn, he, v3 _ _ h he⟩
+        else
+          have : cut (run (run s0 (i + 1)) (n - Nat.succ i)) := by
+            rw [run_run, Nat.add_one, Nat.add_sub_cancel' hn]
+            exact v2 _ hexit
+
+          have ⟨k, _hk, hlek, hck⟩ := find_next_cut_for_cassert s0 (run s0 (i+1)) this
+          have hle' : i + 1 + k ≤ n := by
+            omega
+          have : (cassert s0 (next (run s0 i)) 0).snd := v4 _ _ h he
+          have h' : assert s0 (run s0 (i + 1 + k)) := by
+            rw [run_run] at hck
+            rw [next_run] at this
+            rw [run_run] at hlek
+            simp_all only [Nat.succ_eq_add_one, eq_iff_iff, true_iff]
+            done
           have : n - (i + 1 + k) < n - i := by
             apply Nat.sub_lt_sub_left; assumption; simp_arith
           find (i + 1 + k) h' hle'
